Kroopt/Proofs/Nonces.lean
@@ -60,6 +60,7 @@ theorem successful_open_increments_read_seq
     (hne : s.pendingPlainOut ≠ some b) :
     s'.readEpoch.seq.value = s.readEpoch.seq.value + 1 := by
   unfold handleCryptoResult recordFailAlert at h
+  simp only [] at h
   all_goals (try split at h)
   all_goals (try split at h)
   all_goals (try split at h)
